add a performance test for rsapss

code/experimental/rsapss/c/Hacl_Bignum_Base.c
@@ -1,0 +1,28 @@
+#include <stdint.h>
+#include <immintrin.h>
+#include <x86intrin.h>
+
+#include "Hacl_Bignum_Base.h"
+
+/*
+unsigned char _addcarry_u64 (unsigned char c_in, unsigned __int64 a, unsigned __int64 b, unsigned __int64 * out)
+
+Description
+Add unsigned 64-bit integers a and b with unsigned 8-bit carry-in c_in (carry flag),
+and store the unsigned 64-bit result in out, and the carry-out in dst (carry or overflow flag).
+*/
+
+uint64_t Hacl_Bignum_Base_addcarry_u64_st(uint64_t c_in, uint64_t a, uint64_t b, uint64_t *out) {
+  return _addcarry_u64(c_in, a, b, (long long unsigned int *)out);
+}
+
+/*
+unsigned char _subborrow_u64 (unsigned char b_in, unsigned __int64 a, unsigned __int64 b, unsigned __int64 * out)
+
+Description
+Add unsigned 8-bit borrow b_in (carry flag) to unsigned 64-bit integer b, and subtract the result from
+unsigned 64-bit integer a. Store the unsigned 64-bit result in out, and the carry-out in dst (carry or overflow flag).
+*/
+uint64_t Hacl_Bignum_Base_subborrow_u64_st(uint64_t b_in, uint64_t a, uint64_t b, uint64_t *out) {
+  return _subborrow_u64(b_in, a, b, (long long unsigned int *)out);
+}
