code/experimental/rsapss/Hacl.Bignum.Base.fsti
@@ -29,16 +29,6 @@ val addcarry_u64_st: c_in:carry -> a:uint64 -> b:uint64 -> out:lbuffer uint64 1u
   (ensures  fun h0 c_out h1 -> modifies (loc out) h0 h1 /\
     (c_out, LSeq.index (as_seq h1 out) 0) == addcarry_u64 c_in a b)
 
-[@CInline]
-let addcarry_u64_st c_in a b out =
-  let t1 = a +. c_in in
-  let c = if lt_u64 t1 c_in then u64 1 else u64 0 in
-  let res = t1 +. b in
-  let c = if lt_u64 res t1 then c +. u64 1 else c in
-  out.(0ul) <- res;
-  c
-
-
 (**
 unsigned char _subborrow_u64 (unsigned char b_in, unsigned __int64 a, unsigned __int64 b, unsigned __int64 * out)
 
@@ -52,29 +42,3 @@ val subborrow_u64_st: c_in:carry -> a:uint64 -> b:uint64 -> out:lbuffer uint64 1
   (requires fun h -> live h out)
   (ensures  fun h0 c_out h1 -> modifies (loc out) h0 h1 /\
     (c_out, LSeq.index (as_seq h1 out) 0) == subborrow_u64 c_in a b)
-
-[@CInline]
-let subborrow_u64_st c_in a b out =
-  let res = a -. b -. c_in in
-  let c =
-    if eq_u64 c_in (u64 1) then
-      (if le_u64 a b then u64 1 else u64 0)
-    else
-      (if lt_u64 a b then u64 1 else u64 0) in
-  out.(0ul) <- res;
-  c
-
-
-val mul_carry_add_u64_st: c_in:uint64 -> a:uint64 -> b:uint64 -> out:lbuffer uint64 1ul ->
-  Stack uint64
-  (requires fun h -> live h out)
-  (ensures  fun h0 c_out h1 -> modifies (loc out) h0 h1 /\
-    (c_out, LSeq.index (as_seq h1 out) 0) == mul_carry_add_u64 a b c_in (LSeq.index (as_seq h0 out) 0))
-
-[@CInline]
-let mul_carry_add_u64_st c_in a b out =
-  let d = out.(0ul) in
-  lemma_mul_carry_add_64 a b c_in d;
-  let res = mul64_wide a b +! to_u128 #U64 c_in +! to_u128 #U64 out.(0ul) in
-  out.(0ul) <- to_u64 res;
-  to_u64 (res >>. 64ul)
